src/Bedrock/End2End/X25519/clamp.v
@@ -1,0 +1,152 @@
+From Coq Require Import ZArith Lia. Local Open Scope Z_scope.
+
+Module Z.
+  Lemma testbit_pow2 n i (H : 0 <= n) : Z.testbit (2^n) i = Z.eqb i n.
+  Proof.
+    rewrite <-(Z.mul_1_l (2^n)), Z.mul_pow2_bits by trivial.
+    case (Z.eqb_spec i n) as [->|]; rewrite ?Z.sub_diag; trivial.
+    case (Z.ltb_spec (i-n) 0) as []; rewrite ?Z.testbit_neg_r by lia; trivial.
+    eapply Z.bits_above_log2; cbn; lia.
+  Qed.
+End Z.
+
+Local Ltac t := 
+  try (eapply Z.bits_inj'; intros i Hi);
+  repeat match goal with
+  | _ => progress subst
+  | _ => solve [trivial | lia]
+  | _ => progress rewrite
+       ?Z.sub_simpl_r,
+       ?Z.testbit_0_l, ?Z.testbit_neg_r, ?Z.testbit_pow2, ?Z.testbit_ones,
+       ?Z.lor_spec, ?Z.land_spec, ?Z.lxor_spec, ?Z.ldiff_spec,
+       ?Z.testbit_mod_pow2, ?Z.shiftl_spec, ?Z.shiftl_spec_low, ?Z.shiftr_spec
+       by lia
+  | _ => progress rewrite
+      ?Bool.andb_false_r, ?Bool.andb_true_r,
+      ?Bool.andb_false_l, ?Bool.andb_true_l,
+      ?Bool.orb_false_r, ?Bool.orb_true_r,
+      ?Bool.orb_false_l, ?Bool.orb_true_l,
+      ?Bool.xorb_false_r, ?Bool.xorb_true_r,
+      ?Bool.xorb_false_l, ?Bool.xorb_true_l,
+      ?Bool.negb_involutive
+  | |- _ => progress cbn [negb]
+  | |- context [Z.leb ?x ?y] => destruct (Z.leb_spec x y) as []
+  | |- context [Z.ltb ?x ?y] => destruct (Z.ltb_spec x y) as []
+  | |- context [Z.eqb ?x ?y] => destruct (Z.eqb_spec x y) as []
+  end.
+
+Require Import Crypto.Spec.Curve25519.
+
+Lemma mod8_clamp' k : clamp k mod 8 = 0.
+Proof. cbv [clamp]. Z.div_mod_to_equations. lia. Qed.
+
+Lemma clamp_range k : 2^254 <= clamp k < 2^255.
+Proof. cbv [clamp]. Z.div_mod_to_equations. lia. Qed.
+
+Definition clamp' k := Z.lor (Z.ldiff k (Z.ones 3) mod 2^255) (2^254).
+
+Lemma clamp'_correct k : clamp' k = Curve25519.clamp k.
+Proof.
+  cbv [Curve25519.clamp clamp']; change 8 with (2^3).
+  rewrite Z.mul_comm, <-Z.shiftl_mul_pow2, <-Z.shiftr_div_pow2, ?Z.add_nocarry_lxor; try lia; t.
+Qed.
+
+
+From Coq Require Import ZArith Lia.
+Require Import Coq.Strings.String.
+Require Import Coq.Lists.List.
+Require Import Coq.Init.Byte.
+Require Import bedrock2.Map.Separation.
+Require Import bedrock2.Syntax.
+Require Import bedrock2.NotationsCustomEntry.
+
+Local Open Scope Z_scope.
+Local Open Scope string_scope.
+Import Syntax Syntax.Coercions NotationsCustomEntry.
+Import ListNotations.
+
+Definition clamp := func! (sk) {
+  store1(sk, load1(sk) & $248);
+  store1(sk+$31, (load1(sk+$31) & $127) | $64)
+}.
+
+From coqutil Require Import Word.Interface Word.Naive.
+From coqutil Require Import SortedListWord.
+From coqutil Require Import symmetry.
+Require Import bedrock2.FE310CSemantics.
+Local Existing Instances SortedListString.map SortedListWord.map coqutil.Word.Naive.word.
+
+From coqutil Require Import LittleEndianList.
+Require Import bedrock2.Syntax bedrock2.WeakestPrecondition bedrock2.Map.SeparationLogic.
+Import Coq.Lists.List. (* TODO: SeparationLogic should not override skipn  and etc *)
+From bedrock2 Require Import ProgramLogic. Import ProgramLogic.Coercions.
+Local Notation "m =* P" := ((P%sep) m) (at level 70, only parsing) (* experiment*).
+Local Notation "xs $@ a" := (Array.array ptsto (word.of_Z 1) a xs) (at level 10, format "xs $@ a").
+Import Byte Word.Properties.
+Local Coercion byte.unsigned : byte >-> Z.
+Local Arguments le_combine !_.
+
+Global Instance spec_of_clamp : spec_of "clamp" :=
+  fnspec! "clamp" sk / (s : list Byte.byte) (R : _ -> Prop),
+  { requires t m := m =* s$@sk ⋆ R /\ length s = 32%nat;
+    ensures t' m := t=t' /\ m=* (le_split 32 (Curve25519.clamp (le_combine s)))$@sk ⋆ R }.
+
+Lemma clamp_correct : program_logic_goal_for_function! clamp.
+Proof.
+  straightline; repeat straightline_cleanup.
+
+  do 1 try destruct s as [|?b s]; try (cbn [length] in *; congruence).
+  cbn [Array.array] in *; cbn [length] in *.
+  repeat straightline.
+
+  rewrite <-(firstn_skipn 30 s) in H1 |- *.
+  seprewrite_in @Array.bytearray_append H1; rewrite ?app_length, ?firstn_length_le in * by lia.
+  rewrite <-!Properties.word.add_assoc, <-!Properties.word.ring_morph_add  in *; simpl Z.add in *.
+
+  assert (length (skipn 30 s) = 1)%nat by (rewrite skipn_length; lia). 
+  assert (length (firstn 30 s) = 30)%nat by (rewrite firstn_length; lia). 
+  destruct (skipn 30 s) as [|b31 [] ] eqn:? in *; try (cbn [length] in *; congruence).
+  cbn [Array.array] in *.
+
+  repeat straightline.
+  
+  eassert (Hrw : Lift1Prop.iff1 (ptsto a (Byte.byte.of_Z v0)) ([Byte.byte.of_Z v0]$@a)) by (cbn [Array.array]; cancel).
+  repeat seprewrite_in Hrw H4.
+  repeat seprewrite_in (symmetry! @Array.array_cons) H4.
+  seprewrite_in @Array.bytearray_index_merge H4.
+  { cbn [length]; rewrite ?app_length, ?length_firstn, ?Properties.word.unsigned_of_Z_nowrap; try lia. }
+
+  eassert (le_split _ _ = _) as ->; [|ecancel_assumption].
+  clear -H0 Heql0.
+
+  eapply le_combine_inj; rewrite ?le_combine_split.
+  { repeat (cbn [length]; rewrite ?length_le_split, ?app_length, ?firstn_length). lia. }
+
+  rewrite <-clamp'_correct.
+
+  repeat (cbn [le_combine]; rewrite ?le_combine_app, ?le_combine_firstn).
+
+  subst v v0.
+
+  cbn [length]; rewrite ?firstn_length_le by lia.
+  simpl Z.mul at 1 2.
+  rewrite ?byte.unsigned_of_Z; cbv [byte.wrap].
+  repeat rewrite ?word.unsigned_and_nowrap, ?word.unsigned_or_nowrap.
+
+  pose proof byte.unsigned_range b.
+  pose proof byte.unsigned_range b31.
+  rewrite ?word.unsigned_of_Z_nowrap; try lia.
+  cbv [clamp'].
+
+  rewrite <-(byte.wrap_unsigned b);
+  rewrite <-(byte.wrap_unsigned b31);
+  cbv [byte.wrap].
+  change 127 with (Z.ones 7).
+  change 64 with (2^6).
+  change 248 with (Z.ldiff (Z.ones 8) (Z.ones 3)).
+  change (31%nat * 8) with 248 in *.
+
+  t.
+
+  f_equal; lia.
+Qed.
